Use an interface spec to prove a clean spec
Rewrite TwoDiskProgTheorems.v to re-spec any TwoDiskAPI module.

Some usage of the interface spec, in a manner similar to how we went
from the semantics to a spec with predicates and useful ghost state
(even though for every state, there's a ghost state that makes the
precondition true).

Rather than tying the semantics to [Prim op] as we did before, we will
now tie them to full [prog]s, albeit axiomatic since this is the lowest
level.

src/Shallow/Interface.v
@@ -4,11 +4,15 @@ Require Import ProgLang.Hoare.
 Record InterfaceAPI opT State :=
   { op_sem: forall T, opT T -> Semantics State T; }.
 
-Record InterfaceImpl opT :=
-  { get_op: forall T, opT T -> prog T;
-    (* TODO: add a recovery procedure here *) }.
+Definition background_step {opT State} (bg_step: State -> State -> Prop)
+           (step: forall `(op: opT T), Semantics State T) :=
+  {| op_sem := fun T (op: opT T) state v state'' =>
+                 exists state', bg_step state state' /\
+                       step op state' v state''; |}.
 
-Arguments get_op {opT} impl {T} op : rename.
+Record InterfaceImpl opT :=
+  { op_impl: forall T, opT T -> prog T;
+    (* TODO: add a recovery procedure here *) }.
 
 (* TODO: as with Interpret, this crash spec is nice and all but we really want a
 recovery specification (even for the replicated disk). This also op_spec will
@@ -33,5 +37,14 @@ Record Interface opT State (api: InterfaceAPI opT State) :=
         (* TODO: this atomicity spec is too hard to provide, should prove a
         prog_rok wrt the implementation recovery procedure *)
         prog_ok (op_spec api op)
-                (get_op interface_impl op)
+                (op_impl interface_impl _ op)
                 refinement; }.
+
+Definition get_op opT `{api: InterfaceAPI opT State}
+           (i:Interface api)
+           {T} (op: opT T) : prog T :=
+  op_impl (interface_impl i) _ op.
+
+(* TODO: this coercion works but does not keep T implicit *)
+Coercion get_op : Interface >-> Funclass.
+Add Printing Coercion get_op.
